pcuic/PCUICTranslate.v
@@ -77,8 +77,8 @@ Fixpoint decompose_inductive (ty : type) : option (ename * list type) :=
 
 (** ** Translation of Oak to MetaCoq *)
 
-Definition expr_to_term (Σ : global_env) : expr -> P.term :=
-  fix expr_to_term e :=
+Definition expr_to_term (Σ : global_env) : expr -> term :=
+fix expr_to_term e :=
   match e with
   | eRel i => tRel i
   | eVar nm => tVar nm
@@ -94,16 +94,25 @@ Definition expr_to_term (Σ : global_env) : expr -> P.term :=
   | eConst nm => tConst nm []
   | eCase nm_i ty2 e bs =>
     let (ty1,i) := nm_i in
-    let (nm, tys) := from_option (decompose_inductive ty1) ("Case : not inductive", [tyVar ""]) in
-    let typeInfo := tLambda nAnon (type_to_term ty1) (type_to_term ty2) in
-    let (_,cs) := from_option (resolve_inductive Σ nm) (0,[(nm ++ "not found",[])%string]) in
-    let tbs := map (fun_prod id expr_to_term) bs in
-    let branches := map (trans_branch tys tbs) cs in
-    tCase (mkInd nm 0, i) typeInfo (expr_to_term e) branches
+    let typeInfo := tLambda nAnon (type_to_term ty1)
+                            (lift0 1 (type_to_term ty2)) in
+    match decompose_inductive ty1 with
+    | Some nm_tys =>
+      let (nm, tys) := nm_tys in
+      match (resolve_inductive Σ nm) with
+      | Some v =>
+        let cs := snd v in
+        let tbs := map (fun_prod id expr_to_term) bs in
+        let branches := map (trans_branch tys tbs) cs in
+        tCase (mkInd nm 0, i) typeInfo (expr_to_term e) branches
+      | None => tVar (nm ++ "not found")%string
+      end
+    | None => tVar ("Case : not inductive")%string
+    end
   | eFix nm nv ty1 ty2 b =>
     let tty1 := type_to_term ty1 in
     let tty2 := type_to_term ty2 in
-    let ty := tProd nAnon tty1 tty2 in
+    let ty := tProd nAnon tty1 (lift0 1 tty2) in
     (* NOTE: we have to lift the indices in [tty1] *)
     let body := tLambda (nNamed nv) (lift0 1 tty1) (expr_to_term b) in
     tFix [(mkdef _ (nNamed nm) ty body 0)] 0
